start sketching out code for inodes
just basic stuff for now: iget, iput

similar to Balloc

need to figure out how to go between Rec and a word representation..

src/Inode.v
@@ -11,6 +11,10 @@ Require Import Array.
 Require Import List.
 Require Import Bool.
 Require Import Eqdep_dec.
+Require Import Rec.
+Require Import AddrMap.
+
+Import ListNotations.
 
 Set Implicit Arguments.
 
@@ -23,88 +27,61 @@ Record xparams := {
 }.
 
 Module INODE.
-  Inductive alloc_state :=
-  | Avail
-  | InUse.
+  Definition inodetype : Rec.rectype := [("len", addrlen); ("block0", addrlen)].
+  Definition inode := Rec.recdata inodetype.
 
-  Record inode := mkinode {
-    IFree: alloc_state;
-    ILen: addr;
-    IBlocks: addr -> addr
-  }.
+  Definition inode2valu (i : inode) : valu.
+    (* XXX how to convert a recdata to a word? *)
+  Admitted.
 
-  Definition alloc_state_to_bits a : addr :=
-    match a with
-    | Avail => $0
-    | InUse => $1
-    end.
+  Definition valu2inode (v : valu) : inode.
+    (* XXX how to truncate the 4096-bit valu down to an inode? *)
+  Admitted.
 
-  Definition bits_to_alloc_state (a : addr) : alloc_state :=
-    if (weq a $0) then Avail else InUse.
-
-  Notation "a ^++ b" := (@Word.combine _ a _ b) (at level 55, left associativity).
-
-  Definition inodelen := (addrlen + addrlen + addrlen + addrlen).
-
-  Definition inode_pack (i : inode) : word inodelen :=
-    let (f, l, b) := i in
-    (alloc_state_to_bits f) ^++ l ^++ (b $0) ^++ (b $1).
-
-  Notation "a ^-- sz" := ((@Word.split1 sz _ a), (@Word.split2 sz _ a)) (at level 55).
-
-  Definition inode_unpack (w : word inodelen) : inode :=
-    let (f, w) := w ^-- addrlen in
-    let (l, w) := w ^-- addrlen in
-    let (b0, w) := w ^-- addrlen in
-    let (b1, w) := w ^-- addrlen in
-    mkinode (bits_to_alloc_state f) l
-            (fun x => if weq x $0 then b0 else b1).
-
-  Theorem inode_pack_unpack : forall i,
-    inode_unpack (inode_pack i) = i.
-  Proof.
-    destruct i.
-    unfold inode_unpack, inode_pack.
-    f_equal.
-    (* XXX rewrite split2_combine, split1_combine? *)
-    (* XXX not quite correct because of addrs other than $0 and $1 in IBlocks;
-     * should IBlocks be a fixed-length list instead?  or a list with an extra
-     * Prop field in inode about the length of that list?
-     *)
-  Abort.
-
-  Lemma inodelen_valulen : inodelen + (valulen - inodelen) = valulen.
-  Proof.
-    rewrite valulen_is.
-    auto.
-  Qed.
-
-  Definition inodew2valu (w : word inodelen) : valu.
-    set (zext w (valulen-inodelen)) as r.
-    rewrite inodelen_valulen in r.
-    apply r.
-  Defined.
-
-  Definition valu2inodew (v : valu) : word inodelen.
-    rewrite <- inodelen_valulen in v.
-    apply (split1 inodelen (valulen-inodelen) v).
-  Defined.
-
-  Theorem inodew2valu2inodew : forall i,
-    valu2inodew (inodew2valu i) = i.
-  Proof.
-    unfold valu2inodew, inodew2valu.
-    unfold eq_rec_r, eq_rec.
-    intros.
-    rewrite <- inodelen_valulen.
-    do 2 (rewrite <- eq_rect_eq_dec; try apply eq_nat_dec).
-    apply split1_combine.
-  Qed.
+  Theorem inode2valu2inode: forall i,
+    valu2inode (inode2valu i) = i.
+  Admitted.
 
   Definition rep xp (imap : addr -> inode) :=
     array (IXStart xp)
-          (map (fun i => inode_to_valu (imap $ i)) (seq 0 (wordToNat (IXLen xp)))).
+          (map (fun i => inode2valu (imap $ i)) (seq 0 (wordToNat (IXLen xp)))) $1.
 
+  Definition fupd T (m : addr -> T) a v :=
+    fun a' => if addr_eq_dec a a' then v else m a'.
 
+  Definition iget T lxp xp inum rx : prog T :=
+    v <- LOG.read_array lxp (IXStart xp) inum $1 ;
+    rx (valu2inode v).
+
+  Definition iput T lxp xp inum i rx : prog T :=
+    ok <- LOG.write_array lxp (IXStart xp) inum $1 (inode2valu i) ;
+    rx ok.
+
+  Theorem iget_ok : forall lxp xp inum,
+    {< F mbase m imap,
+    PRE    LOG.rep lxp (ActiveTxn mbase m) *
+           [[ (F * rep xp imap)%pred m ]] *
+           [[ (inum < IXLen xp)%word ]]
+    POST:r LOG.rep lxp (ActiveTxn mbase m) *
+           [[ r = imap inum ]]
+    CRASH  LOG.log_intact lxp mbase
+    >} iget lxp xp inum.
+  Proof.
+    admit.
+  Qed.
+
+  Theorem iput_ok : forall lxp xp inum i,
+    {< F mbase m imap,
+    PRE    LOG.rep lxp (ActiveTxn mbase m) *
+           [[ (F * rep xp imap)%pred m ]] *
+           [[ (inum < IXLen xp)%word ]]
+    POST:r ([[ r = false ]] * LOG.rep lxp (ActiveTxn mbase m)) \/
+           ([[ r = true ]] * exists m', LOG.rep lxp (ActiveTxn mbase m') *
+            [[ (F * rep xp (fupd imap inum i))%pred m ]])
+    CRASH  LOG.log_intact lxp mbase
+    >} iput lxp xp inum i.
+  Proof.
+    admit.
+  Qed.
 
 End INODE.
